\documentclass[10pt]{article}
\title{Solutions to Exercises of Chapter 3}
\author{Ting-Chih Hung \\ \href{mailto:nuit0815@gmail.com}{\texttt{nuit0815@gmail.com}}}
\date{\today}

\usepackage{settings}

\begin{document}
\maketitle

\glsunset{hc}

\section*{Problem 3.1 (Exactness of $p_{\mathrm{FRT}}$)}

\section*{Problem 3.2 (Monte Carlo error of $\hat{p}_{\mathrm{FRT}}$)}

\section*{Problem 3.3 (A finite-sample valid Monte Carlo approximation of $p_{\mathrm{FRT}}$)}

\section*{Problem 3.4 (Fisher's exact test)}

\section*{Problem 3.5 (More details for lady tasting tea)}

\section*{Problem 3.6 (Covariate-adjusted FRT)}

\section*{Problem 3.8 (An algebraic detail)}

We are asked to show that
\begin{align*}
  (n - 1) s^2 
  = \sum_{Z_i = 1} \bp{Y_i - \hat{\bar{Y}}(1)}^2 
    + \sum_{Z_i = 0} \bp{Y_i - \hat{\bar{Y}}(0)}^2
    + \frac{n_1 n_0}{n} \hat{\tau}^2.
  \tag{3.7}
\end{align*}

First,
notice that 
\begin{align*}
  \bar{Y} \equiv \frac{1}{n} \sum_{i=1}^n Y_i 
  = \frac{1}{n} \bp{\sum_{Z_i=1} Y_i + \sum_{Z_i=0} Y_i}
  = \frac{1}{n} \bp{n_1 \hat{\bar{Y}}(1) + n_0 \hat{\bar{Y}}(0)},
\end{align*}
which implies
\begin{align}
  \bar{Y} 
  &= \hat{\bar{Y}}(1) 
  - \frac{n_0}{n} \underbrace{\bp{\hat{\bar{Y}}(1) - \hat{\bar{Y}}(0)}}_{\hat{\tau}}
  = \hat{\bar{Y}}(0)
  + \frac{n_1}{n} \underbrace{\bp{\hat{\bar{Y}}(1) - \hat{\bar{Y}}(0)}}_{\hat{\tau}}. 
    \label{eq:overall-mean}
\end{align}
Therefore, we have
\begin{align*}
  &\mathrel{\phantom{=}} (n - 1) s^2 \\
  &\equiv \sum_{i = 1}^n \bp{Y_i - \bar{Y}}^2 \tag{Definition}\\
  &= \sum_{Z_i = 1} \bp{Y_i - \bar{Y}}^2 + \sum_{Z_i = 0} \bp{Y_i - \bar{Y}}^2 \tag{Partition by $Z_i$} \\
  &= \sum_{Z_i = 1} \bp{Y_i - \hat{\bar{Y}}(1) + \hat{\bar{Y}}(1) - \bar{Y}}^2 
    + \sum_{Z_i = 0} \bp{Y_i - \hat{\bar{Y}}(0) + \hat{\bar{Y}}(0) - \bar{Y}}^2 \tag{Add and subtract} \\
  &= \sum_{Z_i = 1} \bp{Y_i - \hat{\bar{Y}}(1) + \frac{n_0}{n} \hat{\tau}}^2
    + \sum_{Z_i = 0} \bp{Y_i - \hat{\bar{Y}}(0) - \frac{n_1}{n} \hat{\tau}}^2
    \tag{Use \cref{eq:overall-mean}} \\
  &= \sum_{Z_i = 1} \bp{Y_i - \hat{\bar{Y}}(1)}^2 + \frac{n_0^2 n_1}{n^2} \hat{\tau}^2 
    + \sum_{Z_i = 0} \bp{Y_i - \hat{\bar{Y}}(0)}^2 + \frac{n_1^2 n_0}{n^2} \hat{\tau}^2
    \tag{$\sum\limits_{Z_i = z}(Y_i - \hat{\bar{Y}}(z)) = 0$} \\
  &= \sum_{Z_i = 1} \bp{Y_i - \hat{\bar{Y}}(1)}^2 
    + \sum_{Z_i = 0} \bp{Y_i - \hat{\bar{Y}}(0)}^2
    + \frac{n_1 n_0}{n} \hat{\tau}^2,
    \tag{Combine terms}
\end{align*}
which completes the proof.



\printglossaries
\end{document}
